lib/coq/SepBase.v
@@ -15,7 +15,7 @@ License: CC-by 4.0.
 *)
 
 Set Implicit Arguments.
-From CFML Require Export Semantics LibSepFunctor2.
+From CFML Require Export Semantics LibSepFunctor.
 From CFML Require Import LibSepFmap.
 Module Fmap := LibSepFmap.
 Open Scope fmap_scope.
